Checkpoint experimenting with a combination of small step and big step simulation for proving that transaction layer using logging implements banking programs. Reason to experiment is because i have a hard time making pure small step simulation between bank language and logging language work, because the log must contain all writes since the start of the bank program and that seems easier to express in a big-step way than in a small-step way. Also rename Halt in banking language Commit

src/Bank.v
@@ -9,7 +9,7 @@ Section App.
 (* app language *)
 
 Inductive aproc :=
-  | AHalt
+  | ACommit
   | ASetAcct (a:nat) (v:nat) (rx: aproc)
   | AGetAcct (a:nat) (rx: nat->aproc)
   | ATransfer (src:nat) (dst:nat) (v:nat) (rx: aproc)
@@ -17,7 +17,7 @@ Inductive aproc :=
 
 Fixpoint aexec (p:aproc) (s:storage) : storage :=
   match p with
-    | AHalt => s
+    | ACommit => s
     | ASetAcct a v rx => aexec rx (st_write s a v)
     | AGetAcct a rx => aexec (rx (st_read s a)) s
     | ATransfer n m v rx => aexec rx (st_write (st_write s m ((st_read s m) + v)) n ((st_read s n) -v))
@@ -26,7 +26,7 @@ Fixpoint aexec (p:aproc) (s:storage) : storage :=
 Definition initial := 100.
 
 Definition transfer (src:nat) (dst:nat) (v:nat): value * value :=
-  let s := aexec (ASetAcct src initial (ASetAcct dst initial (ATransfer src dst 10 (AHalt)))) st_init in
+  let s := aexec (ASetAcct src initial (ASetAcct dst initial (ATransfer src dst 10 (ACommit)))) st_init in
    (st_read s src, st_read s dst).
 
 (* A simple example to argue that A language is correct *)
@@ -41,28 +41,31 @@ Qed.
 
 (* For small-step simulation in refinement proof of app language to trans language *)
 
+(* XXX not used *)
+
 Record astate := ASt {
   ASProg: aproc;
-  ASDisk: storage
+  ASDisk: storage;
+  ASCommit: bool   (* at beginning of instruction: false; at end of instruction: true *)
 }.
 
 Inductive asmstep : astate -> astate -> Prop :=
-  | AsmHalt: forall d,
-    asmstep (ASt AHalt d) (ASt AHalt d)
+  | AsmCommit: forall d c,
+    asmstep (ASt ACommit d c) (ASt ACommit d true)
   | AsmSetAcct: forall d a v rx,
-    asmstep (ASt (ASetAcct a v rx) d)
-            (ASt rx (st_write d a v))
+    asmstep (ASt (ASetAcct a v rx) d false)
+            (ASt rx (st_write d a v) true)
   | AsmGetAcct: forall d a rx,
-    asmstep (ASt (AGetAcct a rx) d)
-            (ASt (rx (st_read d a)) d)
+    asmstep (ASt (AGetAcct a rx) d false)
+            (ASt (rx (st_read d a)) d true)
   | AsmTransfer: forall d m n v rx,
-    asmstep (ASt (ATransfer m n v rx) d )
+    asmstep (ASt (ATransfer m n v rx) d false)
             (ASt rx (st_write (st_write d m ((st_read d m) - v)) n 
-                    (st_read (st_write d m (st_read d m - v)) n + v)))
+                    (st_read (st_write d m (st_read d m - v)) n + v)) true)
 
     (* must write 3 times, otherwise when m=n the value on disk will
-       depend on arguments' evaluation order *)
-  .
+       depend on arguments' evaluation order *).
+  
 
 End App.
 
